Test/test3.lean
@@ -1,0 +1,10 @@
+import Plausible
+
+/-- error: Found a counter-example! -/
+#guard_msgs in
+example (l1 l2 : List Nat) : l1.length > 0 ∧ l2.length > 0
+  ∧ (l1.all (fun x => decide (x < 10)) = true) ∧ (l2.all (fun x => decide (x < 10)) = true)
+  ∧ (l1.getLast! ≠ 0 ∨ l1 = [0])
+  ∧ (l2.getLast! ≠ 0 ∨ l2 = [0])
+:= by
+  plausible_all (config := {quiet := true})
